proof/asmrefine/SEL4GraphRefine.thy
@@ -10,16 +10,13 @@
 
 theory SEL4GraphRefine
 
-imports "../../tools/asmrefine/GraphRefine"
-  "../../tools/asmrefine/FieldAccessors"
+imports "../../tools/asmrefine/ProveGraphRefine"
   "../../spec/cspec/Substitute"
   "SEL4GlobalsSwap"
 
 begin
 
 ML {* Toplevel.debug := true *}
-
-thm take_heap_list_min
 
 ML {*
 val funs = ParseGraph.funs @{theory} "CFunDump.txt"
@@ -30,6 +27,12 @@ fun define_all funs = fold (fn s => let val s' = Long_Name.base_name s
     val _ = tracing ("defining " ^ s) in
   ParseGraph.define_graph_fun funs (s' ^ "_graph") (Binding.name (s' ^ "_graph_fun")) s end)
   (Symtab.dest funs |> filter (fn (_, v) => #3 v <> NONE) |> map fst)
+*}
+
+ML {*
+val csenv = let
+    val the_csenv = CalculateState.get_csenv @{theory} "c/kernel_all.c_pp" |> the
+  in fn () => the_csenv end
 *}
 
 consts
@@ -47,14 +50,14 @@ lemma eq_impl_at_addrI:
 
 local_setup {* add_field_h_val_rewrites #> add_field_to_bytes_rewrites *}
 
-ML {* val nm = "Kernel_C.getSyscallArg" *}
-
-locale graph_refine = kernel_all_substitute
+locale graph_refine_locale = kernel_all_substitute
     + assumes globals_list_distinct:
         "globals_list_distinct domain symbol_table globals_list"
       assumes halt_halts: "\<exists>ft. (\<forall>s xs. (\<Gamma> \<turnstile> \<langle>com.Call halt_'proc, Normal s\<rangle> \<Rightarrow> xs)
             = (xs = Fault ft))"
 begin
+
+local_setup {* add_globals_swap_rewrites @{thms kernel_all_global_addresses.global_data_mems} *}
 
 definition
   simpl_invariant :: "globals myvars set"
@@ -63,84 +66,113 @@ where
             (hrs_mem (t_hrs_' (globals s)))
         \<and> htd_safe domain (hrs_htd (t_hrs_' (globals s)))}"
 
+ML {* ProveSimplToGraphGoals.test_afll_graph_refine_proofs_after
+    funs (csenv ()) [] @{context} (SOME "Kernel_C.makeUserPDE")  *} 
+
+ML {* val nm = "Kernel_C.makeUserPDE" *}
+
 local_setup {* define_graph_fun_short funs nm *}
 
-ML {* UseHints.globals_swap
+ML {* SimplToGraphProof.globals_swap
  := (fn t => @{term "globals_swap t_hrs_' t_hrs_'_update symbol_table globals_list"} $ t)
 *}
 
 ML {*
-val hints = UseHints.mk_var_deps_hints funs @{context} @{typ "globals myvars"} nm
-*}
-
-ML {* init_graph_refines_proof funs nm @{context} *}
-
-ML {*
-
-val global_data_mems = @{thms kernel_all_global_addresses.global_data_mems[
-       unfolded global_data_defs]}
-
-val pglobal_valids = (*
-(global_data_mems RL
-    @{thms ptr_inverse_safe_htd_safe_global_data[OF globals_list_distinct]
-            ptr_inverse_safe_htd_safe_const_global_data[OF globals_list_distinct]})
-  |> map (full_simplify (HOL_basic_ss addsimps @{thms symbols_in_table_simps
-                    pglobal_valid_fold c_guard_to_word_ineq}))
-  |> map (full_simplify (@{simpset} addsimps @{thms align_td_array' mask_def}))
-*) []
-
-val globals_swap_rewrites2
-    = @{thms globals_list_distinct} RL globals_swap_rewrites
-
+val hints = SimplToGraphProof.mk_hints funs @{context} nm
 *}
 
 ML {*
-mk_graph_refines_proof funs [] hints globals_swap_rewrites2 nm
-  (@{context} addsimps @{thms simpl_invariant_def})
+val init_thm = SimplToGraphProof.simpl_to_graph_upto_subgoals funs [@{thm halt_halts}] hints nm
+    @{context}
 *}
 
-lemma store_word32s_equality_refl:
-  "store_word32s_equality addr xs xs hp hp"
-  by (simp add: store_word32s_equality_def)
+ML {*
+ProveSimplToGraphGoals.simpl_to_graph_thm funs (csenv ()) [@{thm halt_halts}] @{context} nm;
+*}
+
+
+ML {*
+val tacs = ProveSimplToGraphGoals.graph_refine_proof_tacs (csenv ())
+    #> map snd
+val full_tac = ProveSimplToGraphGoals.graph_refine_proof_full_tac
+    (csenv ())
+val full_goal_tac = ProveSimplToGraphGoals.graph_refine_proof_full_goal_tac
+    (csenv ())
+*}
 
 schematic_lemma "PROP ?P"
-  apply (tactic {* rtac it 1 *})
-  apply (tactic {* full_simpl_to_graph_tac funs [] hints nm @{context} *})
-  apply (tactic {* ALLGOALS (TRY o rtac @{thm eq_impl_at_addrI}) *})
-  apply (tactic {* ALLGOALS (simp_tac ((put_simpset HOL_basic_ss @{context})
-      addsimps @{thms mex_def meq_def simpl_invariant_def})) *})
+  apply (tactic {* rtac init_thm 1 *})
+  
+
+  apply (tactic {* ALLGOALS (TRY o (full_goal_tac @{context} THEN_ALL_NEW K no_tac)) *})
+
+(*  apply (tactic {* ALLGOALS (TRY o rtac @{thm eq_impl_at_addrI}) *}) *)
+
+  apply (tactic {* ALLGOALS (nth (tacs @{context}) 0) *})
+apply simp
+  apply (tactic {* ALLGOALS (nth (tacs @{context}) 1) *})
+  apply (tactic {* ALLGOALS (nth (tacs @{context}) 2) *})
 
 
-  apply (tactic {* ALLGOALS (nth (graph_refine_proof_tacs @{context}) 0) *})
-  apply (tactic {* ALLGOALS (nth (graph_refine_proof_tacs @{context}) 1) *})
-  apply (tactic {* ALLGOALS (nth (graph_refine_proof_tacs @{context}) 2) *})
+  apply (tactic {* full_tac @{context} *})
 
-  apply (tactic {* ALLGOALS (simp_tac (@{context} addsimps @{thms
-                       hrs_mem_update
-                       hrs_htd_globals_swap mex_def meq_def}
-                       addsimps globals_swap_rewrites2)) *})
+  apply (simp_all add: word_sle_def[THEN arg_cong[where f=Not], THEN iffD2])
 
-  apply (tactic {* ALLGOALS (nth (graph_refine_proof_tacs @{context}) 3) *})
-  apply (tactic {* ALLGOALS (nth (graph_refine_proof_tacs @{context}) 4) *})
-  apply (tactic {* ALLGOALS (nth (graph_refine_proof_tacs @{context}) 5) *})
-  apply (tactic {* ALLGOALS (nth (graph_refine_proof_tacs @{context}) 6) *})
+defer
+
+  apply (tactic {* full_tac @{context} *})[2]
+
+ML_val {* nth (ProveSimplToGraphGoals.graph_refine_proof_tacs (csenv ()) @{context}) 3 *}
+
+  apply (tactic {* (nth (tacs @{contfext}) 3) 1 *})
 
 
-  apply (simp_all add: field_h_val_rewrites field_to_bytes_rewrites heap_update_def
-                       to_bytes_array upt_rec take_heap_list_min drop_heap_list_general
-                       heap_update_list_append heap_list_update_ptr heap_list_update_word32
-                       store_store_word32_commute_offset field_simps
-                       heap_access_Array_element h_val_word32 h_val_ptr
-                       field_lvalue_offset_eq ucast_eq_0s)
+  apply (tactic {* ProveSimplToGraphGoals.decompose_graph_refine_memory_problems false
+          (@{context} |> Splitter.del_split @{thm split_if}
+        (* |> Simplifier.del_cong @{thm if_weak_cong} *)) 1 *})[1]
 
-  apply (tactic {* simp_tac (@{context} addsimps @{thms store_word32s_equality_fold store_word32s_equality_final add_commute}
-    ) |>ALLGOALS *})
+  apply (tactic {* full_tac @{context} *})[1]
 
-   apply (tactic {* simp_tac (@{context} addsimprocs [store_word32s_equality_simproc]
-    addsimps @{thms store_word32s_equality_final add_commute}
-    ) |>ALLGOALS *})
+  apply (rule sym, tactic {* ProveSimplToGraphGoals.clean_heap_upd_swap @{context} 1 *})
 
-  done
+  apply (tactic {* ProveSimplToGraphGoals.prove_mem_equality @{context} 1 *})
+
+  apply (simp add: heap_update_def to_bytes_array
+               heap_update_list_append heap_list_update_ptr heap_list_update_word32
+               field_lvalue_offset_eq ptr_add_def
+               array_ptr_index_def
+               h_val_word32 h_val_ptr
+               upt_rec take_heap_list_min drop_heap_list_general
+        field_to_bytes_rewrites)
+
+  apply (rule double_heap_update_eq[symmetric])
+
+thm cteInsert_body_def
+
+
+  apply (tafctic {* ALLGOALS (nth (tacs @{context}) 3) *})[1]
+
+  apply (tactic {* ALLGOALS (nth (tacs @{context}) 4) *})
+
+  apply (tactic {* ALLGOALS (nth (tacs @{context}) 5) *})
+
+  apply (tactic {* ALLGOALS (nth (tacs @{context}) 6) *})
+
+  apply (simp_all add: h_val_ptr h_val_word32)
+using [[show_consts]]
+
+term "drop_sign x"
+using [[show_types]]
+thm drop_sign_isomorphism_bitwise(10)[where 'a=32]
+using [[simp_trace]]
+apply (tactic {* ALLGOALS (full_simp_tac (put_simpset HOL_basic_ss @{context}
+      addsimps @{thms drop_sign_isomorphism_bitwise(10)})) *})
+
+
+  apply (tactifc {* ALLGOALS (nth (tacs @{context}) 7) *})
+
+done
+
 
 
 end
