proof/infoflow/Noninterference.thy
@@ -3393,7 +3393,10 @@ lemma cur_domain_reads: "(s,s') \<in> uwr u \<Longrightarrow> is_domain initial_
   prefer 2
   apply simp
   apply (simp add: reads_scheduler_def)+
-  apply (clarsimp simp add: uwr_def sameFor_def sameFor_subject_def)
+  apply (simp add: uwr_def sameFor_def sameFor_subject_def)
+  apply clarify
+  apply (simp(no_asm_use))
+  apply simp
   done
 
 lemmas domain_can_read_context = cur_domain_reads[THEN conjunct1]
