tools/asmrefine/ProveGraphRefine.thy
@@ -1,0 +1,532 @@
+theory ProveGraphRefine
+
+imports GraphRefine
+  GlobalsSwap FieldAccessors
+
+begin
+
+lemma const_globals_in_memory_heap_updateE:
+  "\<lbrakk> globals_list_distinct D symtab gs;
+    const_globals_in_memory symtab gs hmem;
+    htd_safe D htd;
+    ptr_safe (p :: ('a :: wf_type) ptr) htd \<rbrakk>
+     \<Longrightarrow> const_globals_in_memory symtab gs (heap_update p val hmem)"
+  by (simp add: const_globals_in_memory_heap_update)
+
+lemma disjoint_h_val_globals_swap_insert:
+  "\<lbrakk> global_acc_valid g_hrs g_hrs_upd;
+     globals_list_distinct D symtab xs;
+     htd_safe D htd;
+     ptr_safe (p :: ('a :: wf_type) ptr) htd \<rbrakk>
+     \<Longrightarrow> h_val (hrs_mem (g_hrs (globals s))) p
+         = h_val (hrs_mem (g_hrs (globals_swap g_hrs g_hrs_upd symtab xs (globals s)))) p"
+  (* the current apparatus produces goals where the Simpl-derived
+     h_vals are applied to a globals swap and the graph-derived
+     h_vals lack it. we thus *add* a globals swap since that is the
+     case where we can prove ptr_safe *)
+  apply (rule disjoint_h_val_globals_swap[symmetric], assumption+)
+  apply (clarsimp simp: ptr_safe_def htd_safe_def del: subsetI)
+  apply blast
+  done
+
+lemma disjoint_heap_update_globals_swap_rearranged:
+  "\<lbrakk> global_acc_valid g_hrs g_hrs_upd;
+     globals_list_distinct D symtab xs;
+     htd_safe D htd;
+     ptr_safe (p :: ('a :: wf_type) ptr) htd \<rbrakk>
+     \<Longrightarrow> hrs_mem (g_hrs (globals_swap g_hrs g_hrs_upd symtab xs (g_hrs_upd (hrs_mem_update (heap_update p v)) gs)))
+         = heap_update p v (hrs_mem (g_hrs (globals_swap g_hrs g_hrs_upd symtab xs gs)))"
+  apply (subst disjoint_heap_update_globals_swap[symmetric], assumption+)
+   apply (clarsimp simp: ptr_safe_def htd_safe_def del: subsetI)
+   apply blast
+  apply (simp add: global_acc_valid_def hrs_mem_update)
+  done
+
+lemma double_heap_update_eq:
+  "heap_update p' (h_val hp'' p') hp = hp
+    \<Longrightarrow> heap_update p v hp = hp'
+    \<Longrightarrow> (heap_update p v (heap_update p' (h_val hp'' p') hp)) = hp'"
+  by simp
+
+lemma h_t_valid_orig_and_ptr_safe:
+  "h_t_valid d g p \<Longrightarrow> h_t_valid d g p \<and> ptr_safe p d"
+  by (simp add: h_t_valid_ptr_safe)
+
+lemma array_ptr_index_coerce:
+  fixes p :: "(('a :: c_type)['b :: finite]) ptr"
+  shows "n < CARD ('b)
+    \<Longrightarrow> array_ptr_index p False n = array_ptr_index p True n"
+  by (simp add: array_ptr_index_def)
+
+lemma unat_mono_thms:
+  "unat (a + b :: ('a :: len) word) \<le> unat a + unat b"
+  "unat (a * b) \<le> unat a * unat b"
+  by (simp_all add: unat_word_ariths)
+
+lemma unat_mono_intro:
+  "unat a \<le> x \<Longrightarrow> x < b \<Longrightarrow> unat a < b"
+  "unat a \<le> x \<Longrightarrow> x \<le> b \<Longrightarrow> unat a \<le> b"
+  by simp_all
+
+lemma word_neq_0_conv_neg_conv:
+  "(\<not> 0 < (n :: ('a :: len) word)) = (n = 0)"
+  by (cases "n = 0", simp_all)
+
+definition
+  drop_sign :: "('a :: len) signed word \<Rightarrow> 'a word"
+where
+  "drop_sign = ucast"
+
+lemma sint_drop_sign_isomorphism:
+  "sint (drop_sign x) = sint x"
+  by (simp add: drop_sign_def word_sint_msb_eq uint_up_ucast is_up_def
+                source_size_def target_size_def word_size msb_ucast_eq)
+
+lemma drop_sign_isomorphism_ariths:
+  "(x = y) = (drop_sign x = drop_sign y)"
+  "(x < y) = (drop_sign x < drop_sign y)"
+  "(x \<le> y) = (drop_sign x \<le> drop_sign y)"
+  "(x <s y) = (drop_sign x <s drop_sign y)"
+  "(x <=s y) = (drop_sign x <=s drop_sign y)"
+  "drop_sign (x + y) = drop_sign x + drop_sign y"
+  "drop_sign (x - y) = drop_sign x - drop_sign y"
+  "drop_sign (x * y) = drop_sign x * drop_sign y"
+  "drop_sign (- y) = - drop_sign y"
+  "drop_sign (if P then x else y) = (if P then drop_sign x else drop_sign y)"
+  by (simp_all add: drop_sign_def word_less_def
+                    word_le_def word_sless_def word_sle_def
+                    sint_drop_sign_isomorphism[unfolded drop_sign_def]
+                    word_uint.Rep_inject[symmetric]
+                    uint_up_ucast is_up_def source_size_def
+                    target_size_def word_size
+                    uint_word_arith_bintrs
+               del: word_uint.Rep_inject)
+
+lemma drop_sign_isomorphism_bitwise:
+  "drop_sign (x AND y) = drop_sign x AND drop_sign y"
+  "drop_sign (bitOR x y) = bitOR (drop_sign x) (drop_sign y)"
+  "drop_sign (x XOR y) = drop_sign x XOR drop_sign y"
+  "drop_sign (~~ y) = ~~ drop_sign y"
+  "drop_sign (shiftl x n) = shiftl (drop_sign x) n"
+  "drop_sign (shiftr x n) = shiftr (drop_sign x) n"
+  "drop_sign (sshiftr x n) = sshiftr (drop_sign x) n"
+  "drop_sign (ucast z) = ucast z"
+  "drop_sign (scast z) = scast z"
+  "ucast x = ucast (drop_sign x)"
+  "scast x = scast (drop_sign x)"
+  by (rule word_eqI
+          | simp add: word_size drop_sign_def nth_ucast nth_shiftl
+                      nth_shiftr nth_sshiftr word_ops_nth_size
+                      nth_scast
+          | safe
+          | simp add: test_bit_bin)+
+
+lemma drop_sign_number[simp]:
+  "drop_sign (numeral n) = numeral n"
+  "drop_sign (neg_numeral n) = neg_numeral n"
+  "drop_sign 0 = 0" "drop_sign 1 = 1"
+  by (simp_all add: drop_sign_def ucast_def)
+
+lemmas drop_sign_isomorphism
+    = drop_sign_isomorphism_ariths
+        drop_sign_isomorphism_bitwise
+        ucast_id 
+
+lemma ptr_equalities_to_ptr_val:
+  "(Ptr addr = p) = (addr = ptr_val p)"
+  "(p = Ptr addr) = (ptr_val p = addr)"
+  by (simp | cases p)+
+
+(* FIXME move to Lib then to Word *)
+lemmas extra_sle_sless_unfolds
+    = word_sle_def[where a=0 and b=1]
+    word_sle_def[where a=0 and b="numeral n"]
+    word_sle_def[where a=1 and b=0]
+    word_sle_def[where a=1 and b="numeral n"]
+    word_sle_def[where a="numeral n" and b=0]
+    word_sle_def[where a="numeral n" and b=1]
+    word_sless_alt[where a=0 and b=1]
+    word_sless_alt[where a=0 and b="numeral n"]
+    word_sless_alt[where a=1 and b=0]
+    word_sless_alt[where a=1 and b="numeral n"]
+    word_sless_alt[where a="numeral n" and b=0]
+    word_sless_alt[where a="numeral n" and b=1]
+  for n
+
+ML {*
+fun wrap_tac tac i t = let
+    val t' = Goal.restrict i 1 t
+    val r = tac 1 t'
+  in case Seq.pull r of NONE => Seq.empty
+    | SOME (t'', _) => Seq.single (Goal.unrestrict i t'')
+  end
+
+fun eqsubst_wrap_tac ctxt thms = wrap_tac (EqSubst.eqsubst_tac ctxt [0] thms)
+fun eqsubst_asm_wrap_tac ctxt thms = wrap_tac (EqSubst.eqsubst_asm_tac ctxt [0] thms)
+*}
+
+ML {*
+structure ProveSimplToGraphGoals = struct
+
+fun goal_eq (g, g') = 
+    (eq_list (op aconv) (Logic.strip_assums_hyp g, Logic.strip_assums_hyp g'))
+    andalso (Logic.strip_assums_concl g aconv Logic.strip_assums_concl g')
+    andalso (map snd (Logic.strip_params g) = map snd (Logic.strip_params g'))
+
+fun tactic_check s tac = let
+  in fn i => fn t => case Seq.list_of (tac i t)
+    of [] => Seq.empty
+    | [t'] => let
+        val orig_goals = Thm.prems_of t
+        val new_goals = Thm.prems_of t'
+      in (eq_list goal_eq (take (i - 1) orig_goals, take (i - 1) new_goals)
+          andalso eq_list goal_eq (drop i orig_goals,
+              drop (i + length new_goals - length orig_goals) new_goals))
+        orelse raise THM ("tactic " ^ s ^ " broke the rules!", i, [t, t'])
+        ; Seq.single t'
+      end
+    | _ => raise THM ("tactic " ^ s ^ " nondeterministic", i, [t])
+  end
+
+(* FIXME: shadows SimplExport *)
+fun get_c_type_size ctxt (Type (@{type_name array}, [elT, nT])) = 
+    get_c_type_size ctxt elT * Word_Lib.dest_binT nT
+  | get_c_type_size _ @{typ word8} = 1
+  | get_c_type_size _ @{typ word16} = 2
+  | get_c_type_size _ @{typ word32} = 4
+  | get_c_type_size _ @{typ word64} = 8
+  | get_c_type_size _ (Type (@{type_name ptr}, [_])) = 4
+  | get_c_type_size ctxt (T as Type (s, _)) = let
+    val thm = Proof_Context.get_thm ctxt (s ^ "_size")
+      handle ERROR _ => raise TYPE ("get_c_type_size: couldn't get size", [T], [])
+  in Thm.rhs_of thm |> term_of |> HOLogic.dest_number |> snd end
+  | get_c_type_size _ T = raise TYPE ("get_c_type_size:", [T], [])
+
+fun enum_simps csenv ctxt = let
+    val Absyn.CE ecenv = ProgramAnalysis.cse2ecenv csenv;
+  in
+    #enumenv ecenv |> Symtab.dest
+       |> map (Proof_Context.get_thm ctxt o suffix "_def" o fst)
+  end
+
+fun safe_goal_tac ctxt =
+  REPEAT_ALL_NEW (DETERM o CHANGED o safe_steps_tac ctxt)
+
+fun heap_upd_kind (Const (@{const_name heap_update}, _) $ _ $ _ $ _)
+    = "HeapUpd"
+  | heap_upd_kind (Const (@{const_name hrs_mem}, _) $ v)
+    = let
+    val gs = exists_Const (fn (s, _) => s = @{const_name globals_swap}) v
+    val hu = exists_Const (fn (s, _) => s = @{const_name heap_update}) v
+  in (gs orelse raise TERM ("heap_upd_kind: hrs_mem but no globals_swap", [v]));
+    if hu then "HeapUpdWithSwap" else "GlobalUpd"
+  end
+  | heap_upd_kind t = raise TERM ("heap_upd_kind: unknown", [t])
+
+fun except_tac ctxt msg = SUBGOAL (fn (t, _) => let
+  in warning msg; Syntax.pretty_term ctxt t |> Pretty.writeln;
+    raise TERM (msg, [t]) end)
+
+fun res_from_ctxt tac_name thm_name ctxt thm = let
+    val thm_from_ctxt = Proof_Context.get_thm ctxt thm_name
+      handle ERROR _ => raise THM (tac_name ^ ": need thm " ^ thm_name, 1, [])
+  in thm_from_ctxt RS thm
+    handle THM _ => raise THM (tac_name ^ ": need thm to resolve: " ^ thm_name,
+        1, [thm_from_ctxt, thm])
+  end
+
+fun prove_ptr_safe reason ctxt = DETERM o
+    (TRY o REPEAT_ALL_NEW (eqsubst_asm_wrap_tac ctxt
+                @{thms array_ptr_index_coerce}
+            ORELSE' eqsubst_wrap_tac ctxt
+                @{thms array_ptr_index_coerce}
+            )
+        THEN_ALL_NEW asm_simp_tac (ctxt addsimps
+            @{thms ptr_safe_field[unfolded typ_uinfo_t_def]
+                   ptr_safe_Array_element unat_less_helper
+                   h_t_valid_Array_element' h_t_valid_field})
+        THEN_ALL_NEW except_tac ctxt
+            ("prove_ptr_safe: failed for " ^ reason)
+    )
+
+fun get_disjoint_h_val_globals_swap ctxt =
+    @{thm disjoint_h_val_globals_swap_insert}
+        |> res_from_ctxt "prove_heap_update_id" "global_acc_valid" ctxt
+        |> res_from_ctxt "prove_heap_update_id" "globals_list_distinct" ctxt
+
+fun prove_heap_update_id ctxt = DETERM o let
+    val thm = get_disjoint_h_val_globals_swap ctxt
+  in fn i => (resolve_tac @{thms heap_update_id_Array heap_update_id
+                heap_update_id_Array[symmetric] heap_update_id[symmetric]} i
+        ORELSE except_tac ctxt "prove_heap_update_id: couldn't init" i)
+    THEN (simp_tac ctxt
+    THEN_ALL_NEW (* simp_tac will solve goal unless globals swap involved *)
+    ((rtac thm
+      ORELSE' (rtac @{thm sym} THEN' rtac thm)
+      ORELSE' except_tac ctxt "prove_heap_update_id: couldn't rtac")
+    THEN' (atac (* htd_safe assumption *)
+      ORELSE' except_tac ctxt "prove_heap_update_id: couldn't atac")
+    THEN' prove_ptr_safe "prove_heap_update" ctxt)) i
+  end
+
+fun get_field_h_val_rewrites ctxt =
+    Proof_Context.get_thms ctxt "field_h_val_rewrites"
+        handle ERROR _ => raise THM
+            ("run add_field_h_val_rewrites on ctxt", 1, [])
+
+fun get_globals_rewrites ctxt = let
+    val gsr = Proof_Context.get_thms ctxt "globals_swap_rewrites"
+    val cgr = Proof_Context.get_thms ctxt "const_globals_rewrites_with_swap"
+  in (gsr, cgr) end
+        handle ERROR _ => raise THM
+            ("run add_globals_swap_rewrites on ctxt", 1, [])
+
+fun normalise_mem_accs ctxt = DETERM o let
+    val init_simps = @{thms hrs_mem_update
+                       heap_access_Array_element'
+                       o_def
+            } @ get_field_h_val_rewrites ctxt
+        @ #2 (get_globals_rewrites ctxt)
+        @ #1 (get_globals_rewrites ctxt)
+    val h_val = get_disjoint_h_val_globals_swap ctxt
+    val disjoint_h_val_tac
+    = (eqsubst_asm_wrap_tac ctxt [h_val] ORELSE' eqsubst_wrap_tac ctxt [h_val])
+         THEN' (atac ORELSE' except_tac ctxt "normalise_mem_accs: couldn't atac")
+  in
+    asm_full_simp_tac (ctxt addsimps init_simps addsimps [h_val])
+    THEN_ALL_NEW
+        (TRY o REPEAT_ALL_NEW ((eqsubst_wrap_tac ctxt
+                    @{thms heap_access_Array_element'}
+                ORELSE' disjoint_h_val_tac)
+            THEN_ALL_NEW asm_simp_tac (ctxt addsimps init_simps)))
+    THEN_ALL_NEW
+        SUBGOAL (fn (t, i) => case
+            Envir.beta_eta_contract (Logic.strip_assums_concl t)
+          of @{term Trueprop} $ (Const (@{const_name h_t_valid}, _) $ _ $ _ $ _)
+              => prove_ptr_safe "normalise_mem_accs" ctxt i
+            | @{term Trueprop} $ (Const (@{const_name ptr_safe}, _) $ _ $ _)
+              => prove_ptr_safe "normalise_mem_accs" ctxt i
+            | _ => all_tac)
+    THEN_ALL_NEW full_simp_tac (ctxt addsimps @{thms h_val_ptr h_val_word32})
+  end
+
+fun prove_mem_equality ctxt = DETERM o let
+    val init_simpset = ctxt
+        addsimps @{thms hrs_mem_update heap_update_Array_update
+               heap_access_Array_element'
+               o_def
+        } @ get_field_h_val_rewrites ctxt
+    val unpack_simpset = ctxt
+        addsimps @{thms heap_update_def to_bytes_array
+               heap_update_list_append heap_list_update_ptr heap_list_update_word32
+               field_lvalue_offset_eq ptr_add_def
+               array_ptr_index_def
+               h_val_word32 h_val_ptr
+               take_heap_list_min drop_heap_list_general
+        } @ Proof_Context.get_thms ctxt "field_to_bytes_rewrites"
+        addsimprocs [Word_Bitwise_Tac.expand_upt_simproc]
+      handle ERROR _ => raise THM
+        ("prove_mem_equality: run add_field_to_bytes_rewrites on ctxt", 1, [])
+
+    fun double_heap_update_strategy ctxt =
+        resolve_tac @{thms double_heap_update_eq double_heap_update_eq[THEN sym]}
+            THEN' (TRY o SUBGOAL (fn (_, i) => double_heap_update_strategy ctxt i))
+            THEN' prove_heap_update_id ctxt
+
+  in simp_tac init_simpset
+    THEN_ALL_NEW (TRY o REPEAT_ALL_NEW (eqsubst_wrap_tac ctxt
+        @{thms heap_access_Array_element' heap_update_Array_update}))
+    THEN_ALL_NEW TRY o double_heap_update_strategy ctxt
+    THEN_ALL_NEW SUBGOAL (fn (t, i) => if
+        exists_Const (fn (s, T) => s = @{const_name heap_update}
+            andalso get_c_type_size ctxt (domain_type (range_type T)) > 256
+        ) t
+        then except_tac ctxt "prove_mem_equality: unfolding large heap_update" i
+        else all_tac)
+    (* need to normalise mem accs before unfolding unpack_simps
+       as some of this process depends on structured pointer constructions *)
+    THEN_ALL_NEW normalise_mem_accs ctxt
+    THEN_ALL_NEW simp_tac unpack_simpset
+    THEN_ALL_NEW simp_tac (ctxt addsimps @{thms store_word32s_equality_fold
+        store_word32s_equality_final add_commute})
+    THEN_ALL_NEW simp_tac (ctxt addsimprocs [store_word32s_equality_simproc]
+        addsimps @{thms store_word32s_equality_final add_commute})
+    THEN_ALL_NEW SUBGOAL (fn (t, i) => if exists_Const
+            (fn (s, _) => s = @{const_name store_word32}
+                orelse s = @{const_name heap_update}) t
+        then except_tac ctxt "prove_mem_equality: remaining mem upds" i
+        else all_tac)
+  end
+
+fun prove_global_equality ctxt
+    = simp_tac (ctxt addsimps (#1 (get_globals_rewrites ctxt)))
+        THEN' prove_mem_equality ctxt
+
+fun clean_heap_upd_swap ctxt = DETERM o let
+    val thm = @{thm disjoint_heap_update_globals_swap_rearranged}
+    val thm = res_from_ctxt "clean_heap_upd_swap" "global_acc_valid" ctxt thm
+    val thm = res_from_ctxt "clean_heap_upd_swap" "globals_list_distinct" ctxt thm
+  in fn i => rtac @{thm trans}  i
+    THEN (rtac thm i
+      ORELSE except_tac ctxt "clean_heap_upd_swap: couldn't rtac" i)
+    THEN (atac i (* htd_safe assumption *)
+      ORELSE except_tac ctxt "clean_heap_upd_swap: couldn't atac" i)
+    THEN prove_ptr_safe "clean_upd_upd_swap" ctxt i
+  end
+
+fun decompose_mem_goals trace ctxt = SUBGOAL (fn (t, i) =>
+  case Envir.beta_eta_contract (Logic.strip_assums_concl t) of
+    @{term Trueprop} $ (Const (@{const_name const_globals_in_memory}, _) $ _ $ _ $ _)
+        => let val thm = res_from_ctxt "decompose_mem_goals"
+                        "globals_list_distinct" ctxt
+                        @{thm const_globals_in_memory_heap_updateE}
+        in (etac thm THEN' atac THEN' prove_ptr_safe "const_globals" ctxt)
+            ORELSE' except_tac ctxt "decompose_mem_goals: const globals"
+        end i
+    | @{term Trueprop} $ (@{term "op = :: heap_mem \<Rightarrow> _"} $ x $ y) => let
+        val query = (heap_upd_kind x, heap_upd_kind y)
+        val _ = if trace then writeln ("decompose_mem_goals: " ^ @{make_string} query)
+            else ()
+      in case (heap_upd_kind x, heap_upd_kind y) of
+          ("HeapUpd", "HeapUpd") => prove_mem_equality ctxt i
+        | ("HeapUpdWithSwap", "HeapUpd")
+            => clean_heap_upd_swap ctxt i THEN prove_mem_equality ctxt i
+        | ("HeapUpd", "HeapUpdWithSwap") =>
+            rtac @{thm sym} i THEN clean_heap_upd_swap ctxt i THEN prove_mem_equality ctxt i
+        | ("HeapUpd", "GlobalUpd") => prove_global_equality ctxt i
+        | ("GlobalUpd", "HeapUpd") => prove_global_equality ctxt i
+        | _ => raise TERM ("decompose_mem_goals: mixed up "
+            ^ heap_upd_kind x ^ "," ^ heap_upd_kind y, [x, y])
+      end
+    | _ => all_tac)
+
+fun unat_mono_tac ctxt = resolve_tac @{thms unat_mono_intro}
+    THEN' ((((TRY o REPEAT_ALL_NEW (resolve_tac @{thms unat_mono_thms}))
+                THEN_ALL_NEW rtac @{thm order_refl})
+            THEN_ALL_NEW except_tac ctxt "unat_mono_tac: escaped order_refl")
+        ORELSE' except_tac ctxt "unat_mono_tac: couldn't get started")
+    THEN' (asm_full_simp_tac (ctxt addsimps @{thms word_less_nat_alt word_le_nat_alt})
+        THEN_ALL_NEW except_tac ctxt "unat_mono_tac: unsolved")
+
+fun tactic_check' (ss, t) = (ss, tactic_check (hd ss) t)
+
+fun graph_refine_proof_tacs csenv ctxt = let
+    (* FIXME: fix shiftr_no and sshiftr_no in Word *)
+    val ctxt = ctxt delsimps @{thms shiftr_no sshiftr_no}
+        |> Splitter.del_split @{thm split_if}
+        |> Simplifier.del_cong @{thm if_weak_cong}
+
+  in [
+        (["step 1: normalise some word arithmetic. this needs",
+            "to be done before any general simplification.",
+            "also unfold some things that may be in assumptions",
+            "and should be unfolded"],
+        full_simp_tac ((put_simpset HOL_basic_ss ctxt) addsimps @{thms
+              signed_arith_ineq_checks_to_eq_word32
+              signed_arith_eq_checks_to_ord
+              signed_mult_eq_checks32_to_64
+              signed_shift_guard_to_word_32
+              mex_def meq_def}
+              addsimps [Proof_Context.get_thm ctxt "simpl_invariant_def"])),
+        (["step 2: normalise a lot of things that occur in",
+            "simpl->graph that are extraneous"],
+        asm_full_simp_tac (ctxt addsimps @{thms eq_impl_def
+                    var_word32_def var_word8_def var_mem_def
+                    var_htd_def var_acc_var_upd
+                    var_ms_def init_vars_def
+                    return_vars_def upd_vars_def save_vals_def
+                    mem_upd_def mem_acc_def hrs_mem_update
+
+                    (* this includes wrappers for word arithmetic *)
+                    bvlshr_def bvashr_def bvshl_def bv_clz_def
+                    }
+                (* we should also unfold enumerations, since the graph
+                   representation does this, and we need to normalise
+                   word arithmetic the same way on both sides. *)
+                addsimps (enum_simps csenv ctxt)
+            )),
+        (["step 3: split into goals with safe steps",
+            "also derive ptr_safe assumptions from h_t_valid"],
+        (TRY o safe_goal_tac ctxt)
+            THEN_ALL_NEW (TRY o DETERM o REPEAT_ALL_NEW (dtac @{thm h_t_valid_orig_and_ptr_safe}))
+            THEN_ALL_NEW (TRY o safe_goal_tac ctxt)),
+        (["step 4: split up memory write problems."],
+        decompose_mem_goals false ctxt),
+        (["step 5: normalise memory reads"],
+        normalise_mem_accs ctxt),
+        (["step 7: try to simplify out all remaining word logic"],
+        asm_full_simp_tac (ctxt addsimps @{thms
+                        pvalid_def pweak_valid_def palign_valid_def
+                        field_lvalue_offset_eq array_ptr_index_def ptr_add_def
+                        mask_def unat_less_helper
+                        word_sle_def[THEN iffD2] word_sless_alt[THEN iffD2]
+                        field_simps NULL_ptr_val
+                        drop_sign_isomorphism max_word_minus
+                        ptr_equalities_to_ptr_val
+                        extra_sle_sless_unfolds
+                        word_neq_0_conv_neg_conv
+                }
+            )),
+        (["step 8: attack unat less-than properties explicitly"],
+        TRY o unat_mono_tac ctxt)
+
+(* not sure if any of this is useful.
+        asm_full_simp_tac (ctxt addsimps @{thms
+                        to_bytes_array heap_update_def
+                        upt_rec take_heap_list_min drop_heap_list_general
+                        heap_update_list_append heap_list_update_ptr heap_list_update_word32
+                        store_store_word32_commute_offset field_simps
+                        heap_access_Array_element h_val_word32 h_val_ptr
+                        ucast_eq_0s}
+                    addsimps (Proof_Context.get_thms ctxt "field_h_val_rewrites")
+                    addsimps (Proof_Context.get_thms ctxt "field_to_bytes_rewrites")
+                ),
+        simp_tac (ctxt addsimps @{thms store_word32s_equality_fold
+                store_word32s_equality_final add_commute}),
+        simp_tac (ctxt addsimprocs [store_word32s_equality_simproc]
+            addsimps @{thms store_word32s_equality_final add_commute})
+*)
+    ]
+
+  end
+
+fun graph_refine_proof_full_tac csenv ctxt = EVERY
+    (map (fn (ss, t) => ALLGOALS
+        (t ORELSE' except_tac ctxt ("FAILED: " ^ space_implode "\n" ss)))
+        (graph_refine_proof_tacs csenv ctxt))
+
+fun graph_refine_proof_full_goal_tac csenv ctxt
+    = (foldr1 (op THEN_ALL_NEW)
+        (map snd (graph_refine_proof_tacs csenv ctxt)))
+
+fun simpl_to_graph_thm funs csenv noreturns ctxt nm = let
+    val hints = SimplToGraphProof.mk_hints funs ctxt nm
+    val init_thm = SimplToGraphProof.simpl_to_graph_upto_subgoals funs noreturns hints nm
+        ctxt
+    val res_thm = init_thm |> graph_refine_proof_full_tac csenv ctxt |> Seq.hd
+    val _ = if Thm.nprems_of res_thm = 0 then ()
+        else raise THM ("simpl_to_graph_thm: unsolved subgoals", 1, [res_thm])
+    (* FIXME: make hidden assumptions explicit *)
+  in res_thm end
+
+fun test_graph_refine_proof funs csenv noreturns ctxt nm = case
+    Symtab.lookup funs nm of SOME (_, _, NONE) => "skipped " ^ nm
+  | _ => let
+    val ctxt = define_graph_fun_short funs nm ctxt
+  in simpl_to_graph_thm funs csenv noreturns ctxt nm;
+    "success on " ^ nm end
+
+fun test_all_graph_refine_proofs_after funs csenv noreturns ctxt nm = let
+    val ss = Symtab.keys funs
+    val n = case nm of NONE => ~1 | SOME nm' => find_index (fn s => s = nm') ss
+    val ss = if n = ~1 then ss else drop (n + 1) ss
+    val err = prefix "ERROR for: " #> error
+    val _ = map (fn s => (writeln ("testing: " ^ s);
+        writeln (test_graph_refine_proof funs csenv noreturns ctxt s))
+      handle TERM _ => err s | TYPE _ => err s | THM _ => err s) ss
+  in "success" end
+
+end
+*}
+
+end
